move Lib.Loops.Lemmas to Lib.Sequence.Lemmas

lib/Lib.Sequence.Lemmas.fsti
@@ -4,6 +4,7 @@ open FStar.Mul
 open Lib.IntTypes
 open Lib.Sequence
 
+module Loops = Lib.LoopCombinators
 
 #set-options "--z3rlimit 10 --max_fuel 0 --max_ifuel 0 \
               --using_facts_from '-* +Prims +Lib.Sequence.Lemmas +Lib.Sequence'"
@@ -67,3 +68,152 @@ val lemma_map_blocks_vec:
   (ensures
      map_blocks (w * blocksize) inp f_v g_v `Seq.equal`
      map_blocks blocksize inp f g)
+
+
+#reset-options "--z3rlimit 50 --max_fuel 0 --max_ifuel 0"
+
+val repeati_extensionality:
+    #a:Type0
+  -> n:nat
+  -> f:(i:nat{i < n} -> a -> a)
+  -> g:(i:nat{i < n} -> a -> a)
+  -> acc0:a ->
+  Lemma
+  (requires (forall (i:nat{i < n}) (acc:a). f i acc == g i acc))
+  (ensures  (Loops.repeati n f acc0 == Loops.repeati n g acc0))
+
+
+val repeati_right_extensionality:
+    #a:Type
+  -> n:nat
+  -> lo_g:nat
+  -> hi_g:nat{lo_g + n <= hi_g}
+  -> f:(i:nat{i < n} -> a -> a)
+  -> g:(i:nat{lo_g <= i /\ i < hi_g} -> a -> a)
+  -> acc0:a ->
+  Lemma
+  (requires (forall (i:nat{i < n}) (acc:a). f i acc == g (lo_g + i) acc))
+  (ensures (Loops.repeat_right 0 n (Loops.fixed_a a) f acc0 ==
+    Loops.repeat_right lo_g (lo_g + n) (Loops.fixed_a a) g acc0))
+
+
+val repeat_blocks_multi_split:
+     #a:Type0
+  -> #b:Type0
+  -> blocksize:size_pos
+  -> len0:nat{len0 % blocksize = 0}
+  -> inp:seq a{len0 <= length inp /\ length inp % blocksize = 0}
+  -> f:(lseq a blocksize -> b -> b)
+  -> acc0:b ->
+  Lemma
+   (let len = length inp in
+    FStar.Math.Lemmas.modulo_addition_lemma len blocksize (- len0 / blocksize);
+    assert (len % blocksize == (len - len0) % blocksize);
+    repeat_blocks_multi blocksize inp f acc0 ==
+    repeat_blocks_multi blocksize (Seq.slice inp len0 len) f
+      (repeat_blocks_multi blocksize (Seq.slice inp 0 len0) f acc0))
+
+
+val repeat_blocks_split:
+     #a:Type0
+  -> #b:Type0
+  -> blocksize:size_pos
+  -> len0:nat{len0 % blocksize = 0}
+  -> inp:seq a{len0 <= length inp}
+  -> f:(lseq a blocksize -> b -> b)
+  -> l:(len:size_nat{len == length inp % blocksize} -> s:lseq a len -> b -> b)
+  -> acc0:b ->
+  Lemma
+   (let len = length inp in
+    FStar.Math.Lemmas.modulo_addition_lemma len blocksize (- len0 / blocksize);
+    assert (len % blocksize == (len - len0) % blocksize);
+    repeat_blocks blocksize inp f l acc0 ==
+    repeat_blocks blocksize (Seq.slice inp len0 len) f l
+      (repeat_blocks_multi blocksize (Seq.slice inp 0 len0) f acc0))
+
+noextract
+let lanes = w:size_pos{w == 1 \/ w == 2 \/ w == 4}
+
+
+noextract
+let repeat_w (#a:Type0) (w:lanes) (n:nat) (f:(i:nat{i < w * n} -> a -> a)) (i:nat{i < n}) (acc:a) : Tot a =
+  match w with
+  | 1 -> f i acc
+  | 2 -> f (2*i+1) (f (2*i) acc)
+  | 4 -> f (4*i+3) (f (4*i+2) (f (4*i+1) (f (4*i) acc)))
+
+
+val unfold_repeatw:
+    #a:Type0
+  -> w:lanes
+  -> n:pos
+  -> f:(i:nat{i < w * n} -> a -> a)
+  -> acc0:a ->
+  Lemma (Loops.repeati (w*n) f acc0 == repeat_w w n f (n-1) (Loops.repeati (w*(n-1)) f acc0))
+
+
+val lemma_repeati_vec:
+    #a:Type0
+  -> #a_vec:Type0
+  -> w:lanes
+  -> n:nat
+  -> normalize_n:(a_vec -> a)
+  -> f:(i:nat{i < n * w} -> a -> a)
+  -> f_vec:(i:nat{i < n} -> a_vec -> a_vec)
+  -> acc0_vec:a_vec ->
+  Lemma
+  (requires (forall (i:nat{i < n}) (acc_vec:a_vec). normalize_n (f_vec i acc_vec) == repeat_w w n f i (normalize_n acc_vec)))
+  (ensures  (normalize_n (Loops.repeati n f_vec acc0_vec) == Loops.repeati (w * n) f (normalize_n acc0_vec)))
+
+
+private
+val lemma_aux1: w:pos -> blocksize:pos -> len:pos ->
+  Lemma
+  (requires (w * blocksize <= len /\ len % (w * blocksize) = 0 /\ len % blocksize = 0))
+  (ensures  ((len - w * blocksize) / blocksize == w * ((len - w * blocksize) / (w * blocksize))))
+
+
+#set-options "--initial_ifuel 1 --max_ifuel 1"
+
+val lemma_repeat_blocks_multi_vec:
+    #a:Type0
+  -> #b:Type0
+  -> #b_vec:Type0
+  -> w:lanes
+  -> blocksize:size_pos{w * blocksize <= max_size_t}
+  -> inp:seq a{w * blocksize <= length inp /\ length inp % (w * blocksize) = 0 /\ length inp % blocksize = 0}
+  -> f:(lseq a blocksize -> b -> b)
+  -> f_vec:(lseq a (w * blocksize) -> b_vec -> b_vec)
+  -> normalize_n:(b_vec -> b)
+  -> load_acc:(lseq a (w * blocksize) -> b -> b_vec)
+  -> acc0:b ->
+  Lemma
+  (requires
+   (let len = length inp in
+    let len0 = w * blocksize in
+    let len1 = len - len0 in
+    FStar.Math.Lemmas.modulo_addition_lemma len len0 (- 1);
+    assert (len % len0 == len1 % len0);
+    let t0 = Seq.slice inp 0 len0 in
+    let t1 = Seq.slice inp len0 len in
+
+    let nb_vec = len1 / (w * blocksize) in
+    let nb = len1 / blocksize in
+    lemma_aux1 w blocksize len;
+    assert (nb == w * nb_vec);
+    let repeat_bf_vec = repeat_blocks_f (w * blocksize) t1 f_vec nb_vec in
+    let repeat_bf_t0 = repeat_blocks_f blocksize t0 f w in
+    let repeat_bf_t1 = repeat_blocks_f blocksize t1 f nb in
+
+    normalize_n (load_acc t0 acc0) == repeat_w #b w 1 repeat_bf_t0 0 acc0 /\
+    (forall (i:nat{i < nb_vec}) (acc_vec:b_vec).
+      normalize_n (repeat_bf_vec i acc_vec) == repeat_w #b w nb_vec repeat_bf_t1 i (normalize_n acc_vec))))
+  (ensures
+   (let len = length inp in
+    let len0 = w * blocksize in
+    FStar.Math.Lemmas.modulo_addition_lemma len len0 (- 1);
+    assert (len % len0 == (len - len0) % len0);
+
+    let acc_vec = load_acc (Seq.slice inp 0 len0) acc0 in
+    normalize_n (repeat_blocks_multi #a #b_vec (w * blocksize) (Seq.slice inp len0 len) f_vec acc_vec) ==
+    repeat_blocks_multi #a #b blocksize inp f acc0))
